examples/cellio/MainI.v
@@ -22,21 +22,15 @@ Section MainI.
   Definition fnsems :=
     [(MainName.main, (scopes, main))].
 
-  Program Definition Sem: PModSem.t := {|
-    PModSem.scopes := scopes;
-    PModSem.fnsems := fnsems;
-    PModSem.initial_st := [];
+  Program Definition Mod: PMod.t := {|
+    PMod.scopes := scopes;
+    PMod.fnsems := fnsems;
+    PMod.initial_st := [];
   |}
   .
   Solve All Obligations with prove_scope.
   Next Obligation. prove_nodup. Qed.
   
-  Definition Mod: PMod.t := {|
-    PMod.modsem := λ _, Sem;
-    PMod.sk := MainSK.t;
-  |}
-  .
-
   Definition t := Seal.sealing CRIS (PMod.to_hmod Mod).
 
 End MainI. End MainI.
