theories/common/Common.v
@@ -3,5 +3,5 @@ Require Export Program Permutation Orders String HexString ZArith.
 Require Export Axioms Any AList Red IRed SubPerm.
 Require Export sflib Coqlib ITreelib.
 Require Export own SRF invariants sProp syn_invariants.
-Require Export Events Behavior.
+Require Export Events Behavior GEnv.
 
