theories/modules/Spc.v
@@ -1,0 +1,210 @@
+Require Import Common.
+Require Import SMod.
+
+Set Implicit Arguments.
+
+Create HintDb spc.
+Hint Rewrite (Seal.sealing_eq "spc") : spc.
+
+Definition to_spc `{Σ : GRA} (l : alist string fspec) : string -> option fspec :=
+  fun fn => alist_find fn l.
+
+Definition to_spc_context `{Σ : GRA} (spcu : list string) (spck : alist string fspec) :=
+  to_spc (List.map (fun fn => (fn, fspec_trivial)) spcu ++ spck).
+
+Definition to_closed_spc `{Σ : GRA} (l : alist string fspec) : string -> option fspec :=
+  fun fn => match alist_find fn l with
+            | Some fsp => Some fsp
+            | _ => Some fspec_trivial
+            end.
+
+Ltac spc_tac :=
+  match goal with
+  | [ |- to_spc_context _ _ _ = _ ] =>
+    unfold to_spc_context, to_spc;
+    autounfold with spc; autorewrite with spc; simpl
+  | [ |- to_spc ?xs _ = _ ] =>
+    unfold to_spc;
+    autounfold with spc; autorewrite with spc; simpl
+  | [ |- to_closed_spc ?xs _ = _ ] =>
+    unfold to_closed_spc;
+    autounfold with spc; autorewrite with spc; simpl
+  | [ |- alist_find _ ?xs = _ ] =>
+    match type of xs with
+    | (list (string * fspec)) =>
+      autounfold with spc; autorewrite with spc; simpl
+    end
+  | [H : alist_find _ ?xs = _ |- _ ] =>
+    match type of xs with
+    | (list (string * fspec)) =>
+      autounfold with spc in H; autorewrite with spc in H; simpl in H
+    end
+  | [H : to_spc_context _ _ _ = _ |- _ ] =>
+    unfold to_spc_context, to_spc in H;
+    autounfold with spc in H; autorewrite with spc in H; simpl in H
+  | [H : to_spc ?xs _ = _ |- _ ] =>
+    unfold to_spc in H;
+    autounfold with spc in H; autorewrite with spc in H; simpl in H
+  | [H : to_closed_spc ?xs _ = _ |- _ ] =>
+    unfold to_closed_spc in H;
+    autounfold with spc in H; autorewrite with spc in H; simpl in H
+  end.
+
+Section HEADER.
+
+  Context `{Σ: GRA}.
+  
+  Definition fspec_weaker (fsp_src fsp_tgt: fspec): Prop :=
+    forall tid x_src,
+    exists x_tgt,
+      (<<PRE: forall arg_src arg_tgt,
+          (fsp_src.(precond) tid x_src arg_src arg_tgt) ==∗ (fsp_tgt.(precond) tid x_tgt arg_src arg_tgt)>>) ∧
+      (<<POST: forall ret_src ret_tgt,
+          (fsp_tgt.(postcond) tid x_tgt ret_src ret_tgt) ==∗ (fsp_src.(postcond) tid x_src ret_src ret_tgt)>>)
+  .
+
+  Global Program Instance fspec_weaker_PreOrder : PreOrder fspec_weaker.
+  Next Obligation.
+  Proof.
+    ii. exists x_src. esplits; ii.
+    { iStartProof. iIntros "H". iApply "H". }
+    { iStartProof. iIntros "H". iApply "H". }
+  Qed.
+  Next Obligation.
+  Proof.
+    ii. hexploit (H tid x_src). i. des.
+    hexploit (H0 tid x_tgt). i. des. esplits; ii.
+    { iStartProof. iIntros "H".
+      iApply bupd_idemp. iApply PRE0.
+      iApply bupd_idemp. iApply PRE. iApply "H". }
+    { iStartProof. iIntros "H".
+      iApply bupd_idemp. iApply POST.
+      iApply bupd_idemp. iApply POST0. iApply "H". }
+  Qed.
+
+  Variant fn_has_spec (spc : string -> option fspec) (fn : string) (fsp : fspec) : Prop :=
+  | fn_has_spec_intro fsp1
+      (FIND : spc fn = Some fsp1)
+      (WEAK : fspec_weaker fsp fsp1).
+  Hint Constructors fn_has_spec : core.
+
+  Lemma fn_has_spec_weaker (spc : string -> option fspec) (fn : string) (fsp0 fsp1 : fspec)
+      (SPEC : fn_has_spec spc fn fsp1)
+      (WEAK : fspec_weaker fsp0 fsp1) :
+    fn_has_spec spc fn fsp0.
+  Proof. inv SPEC. econs; eauto. etrans; eauto. Qed.
+
+  Definition spc_sub (spc0 spc1 : string -> option fspec) : Prop :=
+    ∀ fn fsp (FIND : spc0 fn = Some fsp), spc1 fn = Some fsp.
+
+  Definition spc_incl (spcl : alist string fspec) (gspc : string -> option fspec) : Prop :=
+    List.NoDup (List.map fst spcl) ∧ spc_sub (to_spc spcl) gspc.
+
+  Global Program Instance spc_sub_PreOrder : PreOrder spc_sub.
+  Next Obligation.
+  Proof. ii. ss. Qed.
+  Next Obligation.
+  Proof. ii. eapply H0, H, FIND. Qed.
+
+  Lemma incl_to_spc spc0 spc1 (INCL : List.incl spc0 spc1)
+        (NODUP : List.NoDup (List.map fst spc1)) :
+      spc_sub (to_spc spc0) (to_spc spc1).
+  Proof.
+    unfold to_spc. ii.
+    eapply alist_find_some in FIND. eapply INCL in FIND.
+    eapply alist_find_some_iff in FIND; et.
+  Qed.
+
+  Lemma to_spc_context_sub spcu spck spcall
+      (INCL : List.incl spck spcall)
+      (NODUP : List.NoDup (spcu ++ (List.map fst spcall))) :
+    spc_sub (to_spc_context spcu spck) (to_closed_spc spcall).
+  Proof.
+    unfold to_spc_context, to_spc, to_closed_spc. ii.
+    rewrite alist_find_app_o in FIND. 
+    destruct (alist_find fn (List.map (fun fn => (fn, fspec_trivial)) spcu)) eqn:EQ; clarify.
+    { eapply alist_find_some in EQ. eapply in_map_iff in EQ. des. clarify.
+      des_ifs. exfalso. eapply alist_find_some in Heq.
+      eapply NoDup_app_disjoint in NODUP; et.
+      eapply in_map with (f:=fst) in Heq. ss. }
+    { eapply alist_find_some in FIND. eapply INCL in FIND.
+      eapply alist_find_some_iff in FIND; et.
+      rewrite FIND; et. eapply nodup_app_r; et. }
+    Unshelve. exact string_Dec.
+  Qed.
+
+  Definition spc_weaker (spc0 spc1 : string -> option fspec) : Prop :=
+    ∀ fn fsp0 (FINDTGT : spc0 fn = Some fsp0),
+      ∃ fsp1, (<<FINDSRC : spc1 fn = Some fsp1>>) ∧ (<<WEAKER : fspec_weaker fsp0 fsp1>>).
+
+  Global Program Instance spc_weaker_PreOrder : PreOrder spc_weaker.
+  Next Obligation. ii. esplits; eauto. refl. Qed.
+  Next Obligation.
+    ii. r in H. r in H0. exploit H; et. intro T; des.
+    exploit H0; et. intro U; des. esplits; eauto. etrans; et.
+  Qed.
+
+  Lemma spc_sub_weaker : spc_sub <2= spc_weaker.
+  Proof.
+    ii. eapply PR in FINDTGT. esplits; et. refl.
+  Qed.
+
+  Lemma incl_spc_sub :
+    ∀ spc0 spc1 (NODUP : List.NoDup (List.map fst spc1)) (INCL : List.incl spc0 spc1),
+      spc_sub (to_spc spc0) (to_spc spc1).
+  Proof.
+    unfold to_spc.
+    ii. eapply alist_find_some in FIND.
+    destruct (alist_find fn spc1) eqn:T.
+    { eapply alist_find_some in T.
+      eapply INCL in FIND.
+      destruct (classic (fsp = f)).
+      { subst. esplits; et. }
+      exfalso.
+      eapply NoDup_inj_aux in NODUP; revgoals.
+      { eapply T. }
+      { eapply FIND. }
+      { ii; clarify. }
+      ss.
+    }
+    eapply alist_find_none in T; et. exfalso. et.
+  Qed.
+
+  Lemma incl_weaker :
+    ∀ spc0 spc1 (NODUP : List.NoDup (List.map fst spc1)) (INCL : List.incl spc0 spc1),
+      spc_weaker (to_spc spc0) (to_spc spc1).
+  Proof. i. eapply spc_sub_weaker. eapply incl_spc_sub; et. Qed.
+
+  Lemma app_sub : ∀ spc0 spc1, spc_sub (to_spc spc0) (to_spc (spc0 ++ spc1)).
+  Proof. unfold to_spc. ii. eapply alist_find_app in FIND. esplits; eauto. Qed.
+
+  Lemma app_weaker : ∀ spc0 spc1, spc_weaker (to_spc spc0) (to_spc (spc0 ++ spc1)).
+  Proof. i. eapply spc_sub_weaker. eapply app_sub. Qed.
+
+  Lemma to_closed_spc_weaker spc : spc_sub (to_spc spc) (to_closed_spc spc).
+  Proof. unfold to_closed_spc, to_spc. ii. rewrite FIND. auto. Qed.
+
+  Lemma incl_to_closed_spc spc0 spc1 (INCL : List.incl spc0 spc1) (NODUP : List.NoDup (List.map fst spc1)) :
+    spc_sub (to_spc spc0) (to_closed_spc spc1).
+  Proof.
+    unfold to_spc, to_closed_spc. ii.
+    eapply alist_find_some in FIND. eapply INCL in FIND.
+    eapply alist_find_some_iff in FIND; et.
+    rewrite FIND. et.
+  Unshelve. exact string_Dec.
+  Qed.
+
+End HEADER.
+
+
+Ltac spc_sub_tac :=
+  i; eapply incl_to_spc;
+  [ autounfold with spc; autorewrite with spc; ii; ss; des; clarify; auto|
+    autounfold with spc; autorewrite with spc; repeat econs; ii; ss; des; ss].
+
+Ltac spc_context_sub_tac :=
+  i; eapply to_spc_context_sub;
+  [ autounfold with spc; autorewrite with spc; ii; ss; des; clarify; auto|
+    autounfold with spc; autorewrite with spc; repeat econs; ii; ss; des; ss].
+
+Ltac ors_tac := repeat ((try by (ss; left; ss)); right).
