theories/simulations/ctxrefine/CtxRefineFacts.v
@@ -1,33 +1,24 @@
 Require Import Common.
-
-Require Import Skeleton Mod HMod.
+Require Import Mod HMod.
 Require Import ModSim ModSimFacts ISimCore ISimFacts.
 Require Import CtxRefine MainAdequacy.
 
 Section CtxRefineFacts.
   Context `{Σ : GRA}.
-  Notation iProp := (iProp Σ).
 
-  Global Program Instance refines_modsem_PreOrder : PreOrder refines_modsem.
+  Global Program Instance refines_mod_PreOrder : PreOrder refines_mod.
   Next Obligation. ii. ss. Qed.
   Next Obligation. ii. eapply H. eapply H0. ss. Qed.
 
   Global Program Instance refines_PreOrder : PreOrder refines.
   Next Obligation.
-    split.
-    { rr. refl. }
     ii. exists rs. esplits; eauto. refl.
   Qed.
   Next Obligation.
-    split.
-    { rr. etrans. apply H. apply H0. }
-    ii. destruct H, H0. des.
-    hexploit (H1 sk); eauto.
-    { etrans; eauto. }
-    i. des.
-    hexploit (H2 sk); eauto.
-    i; des.
-    exists rt0. esplits; eauto.
+    ii.
+    edestruct H; eauto. des.
+    edestruct H0; eauto. des.
+    exists x1. esplits; eauto.
     etrans; eauto.
   Qed.
 
@@ -43,14 +34,13 @@ Section CtxRefineFacts.
   Global Program Instance ctx_refines_Proper : Proper ((≡) ==> (≡) ==> iff) (@ctx_refines Σ).
   Next Obligation.
     intros ms1 ms2 mseq mt1 mt2 mteq; split; intros CTXR;
-      destruct ms1, ms2, mt1, mt2; inv mseq; inv mteq; ss; clarify; econs; ss;
-      specialize (CTXR ctx); inv CTXR; ss;
-      intros sk rs skequiv wfsk wfrs rsimpl wfmod; hexploit (H1 sk rs); eauto.
-    { iIntros "H"; iPoseProof (rsimpl with "H") as "[H1 H2]"; iSplitL "H1"; eauto; iApply H0; ss. }
-    { i; des; esplits; eauto; iIntros "H"; iPoseProof (H4 with "H") as "[H1 H2]";
-        iSplitL "H1"; eauto; iApply H2; ss. }
-    { iIntros "H"; iPoseProof (rsimpl with "H") as "[H1 H2]"; iSplitL "H1"; eauto; iApply H0; ss. }
-    { i; des; esplits; eauto; iIntros "H"; iPoseProof (H4 with "H") as "[H1 H2]";
+      destruct ms1, ms2, mt1, mt2; inv mseq; inv mteq; ss; clarify; ii;
+      specialize (CTXR ctx); ss; hexploit (CTXR rs); eauto.
+    { iIntros "H"; iPoseProof (SRC with "H") as "[H1 H2]"; iSplitL "H1"; eauto; iApply H0; ss. }
+    { i. des; esplits; eauto. iIntros "H". iPoseProof (H1 with "H") as "[H1 H2]".
+      iSplitL "H1"; eauto; iApply H2; ss. }
+    { iIntros "H"; iPoseProof (SRC with "H") as "[H1 H2]"; iSplitL "H1"; eauto; iApply H0; ss. }
+    { i; des; esplits; eauto. iIntros "H"; iPoseProof (H1 with "H") as "[H1 H2]".
         iSplitL "H1"; eauto; iApply H2; ss. }
   Qed.
 
@@ -60,42 +50,38 @@ Section CtxRefineFacts.
     i. specialize (REF HMod.empty_mc).
     destruct mcs, mct. ss.
     rewrite !hmod_add_empty_r in REF.
-    destruct REF. split; eauto.
-    ii. des. ss. hexploit H0; eauto.
+    ii. des. ss. red in REF. hexploit REF; eauto.
     { iIntros "H". iSplit; eauto. iApply SRC. eauto. }
     i; des; esplits; eauto.
-    iIntros "H". iPoseProof (H2 with "H") as "(? & _)". eauto.
+    iIntros "H". iPoseProof (H0 with "H") as "(? & _)". eauto.
   Qed.
 
   (*** weakening for initial condition ***)
-  Lemma ctxr_cond_strengthen (m : HMod.t) (P Q : Sk.t → iProp) (IMPL : ∀ sk, P sk -∗ Q sk) :
+  Lemma ctxr_cond_strengthen (m : HMod.t) (P Q : iProp Σ) (IMPL : P -∗ Q) :
     ctx_refines (m, P) (m, Q).
   Proof.
-    split.
-    - rr. refl.
-    - ii. ss. exists rs. esplits; eauto.
-      + iIntros "H". iPoseProof (SRC with "H") as "(X & Y)".
-        iFrame. iApply IMPL. eauto.
-      + refl.
+    ii. ss. exists rs. esplits; eauto.
+    + iIntros "H". iPoseProof (SRC with "H") as "(X & Y)".
+      iFrame. iApply IMPL. eauto.
+    + refl.
   Qed.
 
   (*** frame rule for initial condition ***)
   Lemma ctxr_cond_frameR (ms mt : HMod.t) Ps Pt Q (REF : ctx_refines (ms, Ps) (mt, Pt)) :
-    ctx_refines (ms, Ps ∗∗ Q)%I (mt, Pt ∗∗ Q)%I.
+    ctx_refines (ms, Ps ∗ Q)%I (mt, Pt ∗ Q)%I.
   Proof.
-    ii. specialize (REF (ctx.1, HMod.addc Q ctx.2)).
-    destruct ctx. unfold HMod.addc in *. ss.
-    destruct REF. split; eauto.
-    ii. ss. des. hexploit H0; eauto.
+    ii. specialize (REF (ctx.1, Q ∗ ctx.2)%I).
+    destruct ctx. ss.
+    ii. ss. des. red in REF. hexploit REF; eauto.
     { iIntros "H". iPoseProof (SRC with "H") as "((? & ?) & ?)".
-      unfold HMod.addc. iFrame. }
+      iFrame. }
     i; des. esplits; eauto.
-    { iIntros "H". iPoseProof (H2 with "H") as "(? & (? & ?))".
-      unfold HMod.addc. iFrame. }
+    { iIntros "H". iPoseProof (H0 with "H") as "(? & (? & ?))".
+      iFrame. }
   Qed.
 
   Lemma ctxr_cond_frameL (ms mt : HMod.t) Ps Pt Q (REF : ctx_refines (ms, Ps) (mt, Pt)) :
-    ctx_refines (ms, Q ∗∗ Ps)%I (mt, Q ∗∗ Pt)%I.
+    ctx_refines (ms, Q ∗ Ps)%I (mt, Q ∗ Pt)%I.
   Proof.
     etrans; [|etrans]; cycle 1.
     { apply ctxr_cond_frameR with (Q:=Q) in REF. apply REF. }
@@ -108,7 +94,7 @@ Section CtxRefineFacts.
     ctx_refines (HMod.add ma mb, P) (HMod.add mb ma, P).
   Proof.
     etrans.
-    { eapply (ctxr_cond_strengthen _ _ (fun sk => (emp ∗ P sk)%I)). eauto. }
+    { eapply (ctxr_cond_strengthen _ _ ((emp ∗ P)%I)). eauto. }
     etrans.
     { eapply ctxr_cond_frameR, main_adequacy, hmod_add_comm. }
     eapply (ctxr_cond_strengthen _ _ P). i. iIntros "(H & H')". iFrame.
@@ -118,7 +104,7 @@ Section CtxRefineFacts.
   Lemma ctxr_frameR ms Ps mt Pt mc (REFA : ctx_refines (ms, Ps) (mt, Pt)) :
     ctx_refines (ms ★ mc, Ps) (mt ★ mc, Pt).
   Proof.
-    ii. specialize (REFA (HMod.add mc ctx.1, ctx.2)). ss.
+    intro. specialize (REFA (HMod.add mc ctx.1, ctx.2)). ss.
     move: REFA; rewrite !hmod_add_assoc; eauto.
   Qed.
 
@@ -134,8 +120,8 @@ Section CtxRefineFacts.
   Lemma ctxr_compose_hor msa Psa mta Pta msb Psb mtb Ptb
       (REFA : ctx_refines (msa, Psa) (mta, Pta))
       (REFB : ctx_refines (msb, Psb) (mtb, Ptb)) :
-    ctx_refines (msa ★ msb, Psa ∗∗ Psb)
-                (mta ★ mtb, Pta ∗∗ Ptb).
+    ctx_refines (msa ★ msb, Psa ∗ Psb)%I
+                (mta ★ mtb, Pta ∗ Ptb)%I.
   Proof.
     etrans.
     - eapply ctxr_frameR, ctxr_cond_frameR. apply REFA.
@@ -146,8 +132,8 @@ Section CtxRefineFacts.
   Lemma ctxr_compose_mix msa Psa mta Pta msb Psb mtb Ptb mc
       (REFA : ctx_refines (msa ★ mc, Psa) (mta ★ mc, Pta))
       (REFB : ctx_refines (msb ★ mc, Psb) (mtb ★ mc, Ptb)) :
-    ctx_refines (msa ★ msb ★ mc, Psa ∗∗ Psb)
-                (mta ★ mtb ★ mc, Pta ∗∗ Ptb).
+    ctx_refines (msa ★ msb ★ mc, Psa ∗ Psb)%I
+                (mta ★ mtb ★ mc, Pta ∗ Ptb)%I.
   Proof.
     etrans.
     { eapply ctxr_frameL, ctxr_cond_frameL. apply REFB. }
